C_Unif_Soundness.v
@@ -1,0 +1,986 @@
+(**
+%\begin{verbatim}
+ ============================================================================
+ Project     : Nominal A, AC and C Unification
+ File        : Soundness.v
+ Authors     : Washington Lu\'is R. de Carvalho Segundo and
+               Mauricio Ayala Rinc\'on 
+               Universidade de Bras\'ilia (UnB) - Brazil
+               Group of Theory of Computation
+ 
+Description : A proof of the soundness of the C-unification algorithm is 
+	      presented in this part of the theory. Roughly speaking, it 
+	      was formalised that each solution of a generated successful 
+	      leaf is also a solution of the original problem.
+ 
+ Last Modified On: November 10th, 2017.
+ ============================================================================
+\end{verbatim}%
+*)
+
+Require Export C_Unif_Termination.
+
+(** %\section{ Soundness of the C-unification algorithm }% *)
+	
+	
+(** %\subsection{ Completeness of fresh\_sys }% *) 
+(**
+	Be a reduction by fresh_sys form T to T'. Sl is a solution
+	for T if and only if Sl a solution for T'. This is proved
+	by case analysis over fresh_sys T T'.
+*) 
+
+Lemma fresh_sys_compl : forall T T' Sl, fresh_sys T T' -> (sol_c Sl T  <-> sol_c Sl T') .
+Proof.
+  intros. destruct T. destruct T'. destruct p. destruct p1.
+  unfold sol_c. simpl. split~; intro H0; destruct H0; destruct H1; destruct H2.
+
+  (* -> *)
+  inverts H; repeat split~; intros.
+    (* fresh_sys_Ut *)
+    apply H1. apply set_remove_1 in H; trivial.
+    apply H2. apply set_remove_1 in H; trivial.
+    (* fresh_sys_At *)
+    apply H1. apply set_remove_1 in H; trivial.
+    apply H2. apply set_remove_1 in H; trivial.
+    (* fresh_sys_Fc *)
+    apply H1 in H5. simpl in H5. inverts H5.
+    case (Constraint_eqdec (a0 #? t) (a #? s1)); intro H9.
+    inverts H9; trivial.
+    apply H1. apply set_remove_1 in H.
+    apply set_add_elim in H. destruct H; try contradiction; trivial.
+    apply H2. apply set_remove_1 in H. apply set_add_elim in H.
+    destruct H; trivial. inverts H.
+    (* fresh_sys_Ab_1 *)
+    apply H1. apply set_remove_1 in H; trivial.
+    apply H2. apply set_remove_1 in H; trivial.
+    (* fresh_sys_Ab_2 *)
+    apply H1 in H11. simpl in H11. inverts H11. false.
+    case (Constraint_eqdec (a0 #? t) (a #? s1)); intro H11.
+    inverts H11; trivial.
+    apply H1. apply set_remove_1 in H.
+    apply set_add_elim in H. destruct H; try contradiction; trivial.
+    apply H2. apply set_remove_1 in H. apply set_add_elim in H.
+    destruct H; trivial. inverts H.
+    (* fresh_sys_Su *)
+    unfold fresh_env in *|-*. intros.
+    apply H1 in H5. simpl in H5.
+    apply fresh_lemma_1 in H5.
+    case ((!pi) $ a ==at a0); intro H6. case (Var_eqdec X X0); intro H7.
+    rewrite <- H6. rewrite <- H7; simpl; autorewrite with perm; trivial.
+    apply H0. apply set_add_elim in H. destruct H; trivial.
+    inverts H. false.
+    apply H0. apply set_add_elim in H. destruct H; trivial.
+    inverts H. false.
+    apply H1. apply set_remove_1 in H; trivial.
+    apply H2. apply set_remove_1 in H; trivial.
+    (* fresh_sys_Pr *)
+    apply H1 in H5. simpl in H5. inverts H5.
+    case (Constraint_eqdec (a0 #? t0) (a #? s1)); intro H11. inverts H11; trivial.
+    case (Constraint_eqdec (a0 #? t0) (a #? t)); intro H12. inverts H12; trivial.
+    apply H1. apply set_remove_1 in H.
+    apply set_add_elim in H. destruct H; try contradiction; trivial.
+    apply set_add_elim in H. destruct H; try contradiction; trivial.
+    apply H2. apply set_remove_1 in H.
+    apply set_add_elim in H. destruct H. inverts H.  
+    apply set_add_elim in H. destruct H; trivial. inverts H.    
+
+  (* <- *)
+  inverts H; repeat split~; intros.
+    (* fresh_sys_Ut *)
+    case (term_eqdec t (<<>>)); intro H6.
+    rewrite H6. simpl. apply fresh_Ut.
+    apply H1. apply set_remove_3; trivial.
+    intro H7. inverts H7. apply H6; trivial.
+    apply H2; apply set_remove_3; trivial.
+    discriminate.
+    (* fresh_sys_At *)
+    case (term_eqdec (%b) t); intro H7.
+    case (a ==at a0); intro H8.
+    rewrite <- H7. rewrite <- H8.
+    simpl. apply fresh_At; trivial.
+    apply H1. apply set_remove_3; trivial.
+    intro H9. inverts H9. apply H8; trivial.
+    apply H1. apply set_remove_3; trivial.
+    intro H9. inverts H9. apply H7; trivial.
+    apply H2; apply set_remove_3; trivial.
+    discriminate.
+    (* fresh_sys_Fc *)
+    assert (Q : fst Sl |- a # (Fc E n (s1 |^ snd Sl))).
+     apply fresh_Fc. apply H1. apply set_remove_3.
+     apply set_add_intro2; trivial.     
+     intro H'. inverts H'. symmetry in H6.
+     apply Fc_neq_psub in H6; trivial.
+    case (term_eqdec (Fc E n s1) t); intro H7.
+    case (a ==at a0); intro H9.
+    rewrite <- H7. rewrite <- H9. simpl; trivial.
+    apply H1. apply set_remove_3.
+    apply set_add_intro1; trivial.
+    intro H10. inverts H10. apply H9; trivial.
+    apply H1. apply set_remove_3.
+    apply set_add_intro1; trivial.
+    intro H10. inverts H10. apply H7; trivial.
+    apply H2; apply set_remove_3.
+    apply set_add_intro1; trivial.
+    discriminate.    
+    (* fresh_sys_Ab_1 *)
+    case (term_eqdec ([a]^s1) t); intro H6.
+    case (a ==at a0); intro H7.
+    rewrite <- H6. rewrite <- H7.
+    simpl. apply fresh_Ab_1; trivial.
+    apply H1. apply set_remove_3; trivial.
+    intro H9. inverts H9. apply H7; trivial.
+    apply H1. apply set_remove_3; trivial.
+    intro H9. inverts H9. apply H6; trivial.
+    apply H2; apply set_remove_3; trivial.
+    discriminate.
+    (* fresh_sys_Ab_2 *)
+    assert (Q : fst Sl |- a # ([b]^(s1 |^ snd Sl))).
+     apply fresh_Ab_2; trivial.
+     apply H1. apply set_remove_3.
+     apply set_add_intro2; trivial.     
+     intro H'. inverts H'. symmetry in H5.
+     apply Ab_neq_psub in H5; trivial.
+    case (term_eqdec ([b]^s1) t); intro H7.
+    case (a ==at a0); intro H9.
+    rewrite <- H7. rewrite <- H9. simpl; trivial.
+    apply H1. apply set_remove_3.
+    apply set_add_intro1; trivial.
+    intro H10. inverts H10. apply H9; trivial.
+    apply H1. apply set_remove_3.
+    apply set_add_intro1; trivial.
+    intro H10. inverts H10. apply H7; trivial.
+    apply H2; apply set_remove_3.
+    apply set_add_intro1; trivial.
+    discriminate.
+    (* fresh_sys_Su *)
+    unfold fresh_env in *|-*. intros.
+    apply H0. apply set_add_intro1; trivial.
+    case (term_eqdec (pi|.X) t); intro H6.
+    case (a ==at a0); intro H7.
+    rewrite <- H6. rewrite <- H7.
+    replace (pi|.X) with (pi @ ([]|.X)).
+    rewrite subst_perm_comm.
+    gen_eq pi' : (!pi); intro H8.
+    replace pi with (!pi').
+    apply fresh_lemma_2. unfold fresh_env in H0.
+    apply H0. apply set_add_intro2; trivial.
+    rewrite H8. apply rev_involutive.
+    autorewrite with perm. simpl. trivial.
+    apply H1. apply set_remove_3; trivial.
+    intro H8. inverts H8. apply H7; trivial.
+    apply H1. apply set_remove_3; trivial.
+    intro H7. inverts H7. apply H6; trivial.
+    apply H2. apply set_remove_3; trivial.
+    discriminate.    
+    (* fresh_sys_Pr *)
+    assert (Q : fst Sl |- a # (<| s1|^(snd Sl), t|^(snd Sl)|>)).
+     apply fresh_Pr.
+     apply H1. apply set_remove_3.
+     apply set_add_intro1. apply set_add_intro2; trivial.    
+     intro H'. inverts H'. apply symmetry in H6.
+     apply Pr_neq_psub_1 in H6; trivial.     
+     apply H1. apply set_remove_3.
+     apply set_add_intro2; trivial.    
+     intro H'. inverts H'. apply symmetry in H6.
+     apply Pr_neq_psub_2 in H6; trivial. 
+    case (term_eqdec (<|s1,t|>) t0); intro H6.
+    case (a ==at a0); intro H7.
+    rewrite <- H6. rewrite <- H7. simpl; trivial.
+    apply H1. apply set_remove_3.
+    apply set_add_intro1. apply set_add_intro1; trivial.
+    intro H8. inverts H8. apply H7; trivial.
+    apply H1. apply set_remove_3.
+    apply set_add_intro1. apply set_add_intro1; trivial.
+    intro H8. inverts H8. apply H6; trivial.
+    apply H2; apply set_remove_3.
+    apply set_add_intro1. apply set_add_intro1; trivial.
+    discriminate. 
+Qed.  
+
+(** %\subsection{ Preservation of solutions by equ\_sys }% *) 
+(**
+	Be a reduction by equ_sys form T to T'. If Sl is a solution
+	for T', then Sl is also a solution for T. This is proved
+	by case analysis over equ_sys T T'.
+*)    
+
+Lemma equ_sol_preserv : forall T T' Sl varSet, valid_triple T ->
+                        equ_sys varSet T T' -> sol_c Sl T' -> sol_c Sl T .
+Proof.
+  intros. destruct T. destruct T'. destruct p. destruct p1.
+  unfold sol_c in *|-*. destruct Sl. simpl in *|-*.
+  destruct H1. destruct H2. destruct H3. 
+  inverts H0; repeat split~; intros.  
+
+  (* equ_sys_refl *)
+
+  apply H2. apply set_remove_3; trivial. discriminate.
+  case (term_eqdec s t); intro H5. rewrite H5. apply c_equiv_refl.
+  apply H3. apply set_remove_3; trivial. intro H7. inverts H7.
+  apply H5; trivial.
+
+  (* equ_sys_Pr *)
+
+  apply H2. apply set_remove_3.
+  apply set_add_intro1. apply set_add_intro1; trivial.
+  discriminate.
+  assert (Q: c1 |- <|s2,s3|>|^s1 ~c (<|t0,t1|>|^s1)).
+   simpl. apply equiv_Pr.
+   apply H3. apply set_remove_3. 
+   apply set_add_intro1. apply set_add_intro2; trivial.
+   intro H7. inverts H7. symmetry in H8.
+   apply Pr_neq_psub_1 in H8. trivial.
+   apply H3. apply set_remove_3. 
+   apply set_add_intro2; trivial.
+   intro H7. inverts H7. symmetry in H8.
+   apply Pr_neq_psub_2 in H8. trivial.   
+  case (Constraint_eqdec (s~?t) ((<|s2,s3|>)~?(<|t0,t1|>))); intro H7.
+  inverts H7; trivial.
+  apply H3. apply set_remove_3; trivial.
+  apply set_add_intro1. apply set_add_intro1; trivial. 
+
+  (* equ_sys_Fc *)
+
+  apply H2. apply set_remove_3. apply set_add_intro1; trivial.
+  discriminate.
+  assert (Q : c1 |- (t|^s1) ~c (t'|^s1)).
+   apply H3. apply set_remove_3. apply set_add_intro2; trivial.
+   intro H8. inverts H8. symmetry in H6.
+   apply Fc_neq_psub in H6. trivial.
+  case (Constraint_eqdec (s~?t0) ((Fc E n t)~?(Fc E n t'))); intro H8.
+  inverts H8. apply c_equiv_Fc; trivial.
+  apply H3. apply set_remove_3.
+  apply set_add_intro1; trivial.
+  intro H9. inverts H9. apply H8; trivial.
+  
+  (* equ_sys_C1 *)
+
+  apply H2. apply set_remove_3. 
+  apply set_add_intro1. apply set_add_intro1; trivial.
+  discriminate.
+  assert (Q: c1 |- <|s2,s3|>|^s1 ~c (<|t0,t1|>|^s1)).
+   simpl. apply equiv_Pr.
+   apply H3. apply set_remove_3. 
+   apply set_add_intro1. apply set_add_intro2; trivial.
+   intro H7. inverts H7. symmetry in H8.
+   apply Fc_Pr_neq_psub_1 in H8. trivial.
+   apply H3. apply set_remove_3. 
+   apply set_add_intro2; trivial.
+   intro H7. inverts H7. symmetry in H8.
+   apply Fc_Pr_neq_psub_2 in H8. trivial.   
+  case (Constraint_eqdec (s~?t) (Fc 2 n (<|s2,s3|>)~?(Fc 2 n (<|t0,t1|>)))); intro H7.
+  inverts H7. simpl in Q|-*. apply c_equiv_Fc; trivial. 
+  apply H3. apply set_remove_3; trivial.
+  apply set_add_intro1. apply set_add_intro1; trivial. 
+  
+  (* equ_sys_C2 *)
+
+  apply H2. apply set_remove_3. 
+  apply set_add_intro1. apply set_add_intro1; trivial.
+  discriminate.
+  assert (Q: c1 |- <|s2,s3|>|^s1 ~c (<|t1,t0|>|^s1)).
+   simpl. apply equiv_Pr.
+   apply H3. apply set_remove_3. 
+   apply set_add_intro1. apply set_add_intro2; trivial.
+   intro H7. inverts H7. symmetry in H8.
+   apply Fc_Pr_neq_psub_1 in H8. trivial.
+   apply H3. apply set_remove_3. 
+   apply set_add_intro2; trivial.
+   intro H7. inverts H7. symmetry in H8.
+   apply Fc_Pr_neq_psub_2 in H8. trivial.   
+  case (Constraint_eqdec (s~?t) (Fc 2 n (<|s2,s3|>)~?(Fc 2 n (<|t0,t1|>)))); intro H7.
+  inverts H7. simpl in Q|-*. inverts Q. apply equiv_C2; trivial. left~.
+  apply H3. apply set_remove_3; trivial.
+  apply set_add_intro1. apply set_add_intro1; trivial. 
+
+
+  (* equ_sys_Ab1 *)
+
+  apply H2. apply set_remove_3. apply set_add_intro1; trivial.
+  discriminate.
+  assert (Q: c1 |- t|^s1 ~c (t'|^s1)).
+   apply H3. apply set_remove_3. 
+   apply set_add_intro2; trivial.
+   intro H5. inverts H5. symmetry in H8.
+   apply Ab_neq_psub in H8. trivial.
+  case (Constraint_eqdec (s~?t0) (([a]^t) ~? ([a]^t'))); intro H7.
+  inverts H7. simpl. apply equiv_Ab_1; trivial.
+  apply H3. apply set_remove_3; trivial.
+  apply set_add_intro1; trivial.
+
+
+  (* equ_sys_Ab2 *) 
+  apply H2. apply set_remove_3.
+  apply set_add_intro1. apply set_add_intro1; trivial.
+  discriminate.
+  assert (Q : c1 |- t|^s1 ~c ((([(a, b)]) @ t')|^s1)).
+   apply H3. apply set_remove_3.
+   apply set_add_intro1. apply set_add_intro2; trivial. 
+   intro H5. inverts H5. symmetry in H8.
+   apply Ab_neq_psub in H8. trivial.
+  assert (Q' : c1 |- a # (t'|^s1)).
+   apply H2. apply set_remove_3.
+   apply set_add_intro2; trivial.
+   discriminate.
+  case (Constraint_eqdec (s~?t0) (([a]^t) ~? ([b]^t'))); intro H8.
+  inverts H8. simpl. apply equiv_Ab_2; trivial.
+  rewrite <- subst_perm_comm; trivial.
+  apply H3. apply set_remove_3; trivial.
+  apply set_add_intro1. apply set_add_intro1; trivial.
+
+
+  (* equ_sys_inst *)
+
+  assert (Q : c1 |- a # (t0|^(([(X,(!pi)@t)]©s1)))).
+   rewrite subst_comp_expand. apply H2.
+   apply set_union_intro1.
+   replace (a #? (t0 |^ ([(X, (! pi) @ t)]))) with (subs_Constraint (a#?t0) ([(X, (! pi) @ t)])).
+   apply set_In_subs_problem. apply set_remove_3. apply set_remove_3; trivial.
+   intro H10. inverts H10. intro H10. inverts H10.
+   simpl; trivial.
+
+  assert (Q': set_In X (Problem_vars p0)).
+   destruct H12. apply Problem_vars_set_In with (u:= (pi|.X)~?t); trivial.
+   simpl. apply set_union_intro1. left~.
+   apply Problem_vars_set_In with (u:= t~?(pi|.X)); trivial.
+   simpl. apply set_add_intro2; trivial.
+
+  assert (Q'': forall Y, set_In Y (term_vars t) ->  set_In Y (Problem_vars p0)).
+   intros. destruct H12. apply Problem_vars_set_In with (u:= (pi|.X)~?t); trivial.
+   simpl. apply set_union_intro2; trivial.
+   apply Problem_vars_set_In with (u:= t~?(pi|.X)); trivial.
+   simpl. apply set_add_intro1; trivial.
+  
+   
+  clear H0 H1 H2 H3 H12.
+
+  induction t0; simpl in *|-*; trivial.
+  case (a ==at a0); intro H2. rewrite H2. apply fresh_Ab_1.
+  apply fresh_Ab_2; trivial. apply IHt0.
+  inverts Q. false. trivial.
+  inverts Q. apply fresh_Pr.
+  apply IHt0_1; trivial. apply IHt0_2; trivial.
+  inverts Q. apply fresh_Fc. apply IHt0; trivial.
+  
+  gen Q. case (X ==v v); trivial. intros H2 Q.
+  rewrite <- H2. clear H2.
+  apply c_equiv_fresh with (t1:= p @ (((! pi) @ t) |^ s1)); trivial.
+  apply c_equiv_equivariance. replace (look_up X s1) with (([]|.X)|^s1).
+  case H4; clear H4; intros s2 H4.
+  apply c_equiv_unif_2 with (S1:=(s©([(X,(!pi) @ t)]))©s2); trivial.
+  unfold valid_triple in H. simpl in H. destruct H.
+  rewrite 4 subst_comp_expand.
+  rewrite 2 inter_dom_term_vars with (t:= (!pi)@t).
+  rewrite not_In_dom. rewrite subst_var_eq.
+  autorewrite with perm. apply c_equiv_refl.
+  intro H5. apply set_inter_nil with (a:=X) in H.
+  apply H. apply set_inter_intro; trivial.
+  apply In_dom_eq_dom_rec; trivial. 
+  apply set_inter_nil; intros. intro H1.
+  apply set_inter_elim in H1. destruct H1.
+  apply var_in_dom_rec_singleton in H2.
+  rewrite H2 in H1. rewrite perm_term_vars in H1.
+  apply H9. apply set_union_intro1; trivial.
+  apply set_inter_nil; intros. intro H5.
+  apply set_inter_elim in H5. destruct H5.
+  apply set_inter_nil with (a:=a0) in H. apply H.
+  apply set_inter_intro; trivial.
+  rewrite perm_term_vars in H1. apply Q''; trivial.
+  simpl. autorewrite with perm; trivial.
+
+  assert (Q1: forall Y, set_In Y (term_vars t) ->  set_In Y (Problem_vars p0)).
+   intros. destruct H12. apply Problem_vars_set_In with (u:= (pi|.X)~?t); trivial.
+   simpl. apply set_union_intro2; trivial.
+   apply Problem_vars_set_In with (u:= t~?(pi|.X)); trivial.
+   simpl. apply set_add_intro1; trivial.
+   
+  assert (Q2: forall Y, set_In Y (term_vars t0) ->  set_In Y (Problem_vars p0)).
+   intros. apply Problem_vars_set_In with (u:= s0~?t0); trivial.
+   simpl. apply set_union_intro2; trivial.
+
+  assert (Q3: forall Y, set_In Y (term_vars s0) ->  set_In Y (Problem_vars p0)).
+   intros. apply Problem_vars_set_In with (u:= s0~?t0); trivial.
+   simpl. apply set_union_intro1; trivial.
+
+  case H4; clear H4; intros s2 H4.
+  unfold valid_triple in H; simpl in H. destruct H.
+  
+  case (Constraint_eqdec (s0~?t0) ((pi|.X)~?t)); intro H6. inverts H6.
+
+  apply c_equiv_unif_2 with (S1:=(s©([(X,(!pi) @ t)]))©s2); trivial.
+  rewrite 4 subst_comp_expand.
+  rewrite not_In_dom. rewrite subst_var_eq.
+  rewrite inter_dom_term_vars with (t:= t).
+  rewrite not_occurs; trivial.
+  rewrite 2 subst_perm_comm.
+  apply c_equiv_pi_inv_side. apply c_equiv_refl.
+  intro H10. apply H9. apply set_union_intro1; trivial.
+  apply set_inter_nil; intros. intro H8.
+  apply set_inter_elim in H8. destruct H8.
+  apply set_inter_nil with (a:=a) in H. apply H.
+  apply set_inter_intro; trivial.
+  apply Q2; trivial. intro H8.
+  apply set_inter_nil with (a:=X) in H. apply H.
+  apply set_inter_intro. apply In_dom_eq_dom_rec; trivial.
+  apply Q3. simpl. left~.
+
+  case (Constraint_eqdec (s0~?t0) (t~?(pi|.X))); intro H7. inverts H7. 
+
+  apply c_equiv_unif_2 with (S1:=(s©([(X,(!pi) @ t)]))©s2); trivial.
+  rewrite 4 subst_comp_expand.
+  rewrite not_In_dom. rewrite subst_var_eq.
+  rewrite inter_dom_term_vars with (t:= t).
+  rewrite not_occurs; trivial.
+  rewrite 2 subst_perm_comm. apply c_equiv_sym.
+  apply c_equiv_pi_inv_side. apply c_equiv_refl.
+  intro H10. apply H9. apply set_union_intro1; trivial.
+  apply set_inter_nil; intros. intro H8.
+  apply set_inter_elim in H8. destruct H8.
+  apply set_inter_nil with (a:=a) in H. apply H.
+  apply set_inter_intro; trivial.
+  apply Q1; trivial. intro H8.
+  apply set_inter_nil with (a:=X) in H. apply H.
+  apply set_inter_intro. apply In_dom_eq_dom_rec; trivial.
+  apply Q2. simpl. left~.
+  
+  assert (Q : c1 |- (s0|^(([(X,(!pi)@t)]©s1))) ~c (t0|^(([(X,(!pi)@t)]©s1)))).
+   rewrite 2 subst_comp_expand. apply H3.
+   apply set_union_intro1.
+   replace ((s0 |^ ([(X, (! pi) @ t)])) ~? (t0 |^ ([(X, (! pi) @ t)])))
+     with (subs_Constraint (s0~?t0) ([(X, (! pi) @ t)])).
+   apply set_In_subs_problem. apply set_remove_3; trivial. apply set_remove_3; trivial.
+   simpl; trivial.
+
+  clear H0 H1 H2 H3 H5 H6 H7 H12.
+  rewrite 2 subst_comp_expand in Q.
+  apply c_equiv_unif_2 with (S1 := (s © ([(X, (! pi) @ t)])) © s2); trivial.
+  apply c_equiv_unif_2 with (S2 := (s © ([(X, (! pi) @ t)])) © s2) in Q. clear H4.
+  rewrite 4 subst_comp_expand in Q.  rewrite 4 subst_comp_expand.
+  rewrite inter_dom_term_vars with (t:= s0).
+  rewrite inter_dom_term_vars with (t:= t0).
+  rewrite 2 inter_dom_term_vars with (S:= s) in Q.
+  rewrite inter_dom_term_vars with (t:= s0 |^ ([(X, (! pi) @ t)])) in Q.
+  rewrite inter_dom_term_vars with (t:= t0 |^ ([(X, (! pi) @ t)])) in Q. trivial.
+
+  clear Q.
+  apply set_inter_nil; intros. intro H0.
+  apply set_inter_elim in H0. destruct H0.
+  apply var_in_dom_rec_singleton in H1.
+  rewrite H1 in H0. apply In_im_subst_term in H0.
+  rewrite perm_term_vars in H0.
+  apply H9. apply set_union_intro1; trivial.
+
+  clear Q.
+  apply set_inter_nil; intros. intro H0.
+  apply set_inter_elim in H0. destruct H0.
+  apply var_in_dom_rec_singleton in H1.
+  rewrite H1 in H0. apply In_im_subst_term in H0.
+  rewrite perm_term_vars in H0.
+  apply H9. apply set_union_intro1; trivial.
+
+  clear Q.
+  apply set_inter_nil; intros. intro H0.
+  apply set_inter_elim in H0. destruct H0.  
+  apply set_inter_nil with (a:=a) in H.
+  apply H. apply set_inter_intro; trivial.
+  apply In_im_subst_term' in H0.
+  apply set_union_elim in H0. destruct H0.
+  apply Q2; trivial.
+  rewrite perm_term_vars in H0.
+  apply Q1; trivial.
+
+  clear Q.
+  apply set_inter_nil; intros. intro H0.
+  apply set_inter_elim in H0. destruct H0.  
+  apply set_inter_nil with (a:=a) in H.
+  apply H. apply set_inter_intro; trivial.
+  apply In_im_subst_term' in H0.
+  apply set_union_elim in H0. destruct H0.
+  apply Q3; trivial.
+  rewrite perm_term_vars in H0.
+  apply Q1; trivial.
+ 
+  clear Q.
+  apply set_inter_nil; intros. intro H0.
+  apply set_inter_elim in H0. destruct H0.  
+  apply set_inter_nil with (a:=a) in H.
+  apply H. apply set_inter_intro; trivial.
+  apply Q2; trivial.
+
+  clear Q.
+  apply set_inter_nil; intros. intro H0.
+  apply set_inter_elim in H0. destruct H0.  
+  apply set_inter_nil with (a:=a) in H.
+  apply H. apply set_inter_intro; trivial.
+  apply Q3; trivial.
+
+  apply subst_sym; trivial.
+
+  case H4; clear H4; intros s2 H4.
+  exists ([(X,(!pi)@t)] © s2).
+  apply subst_assoc; trivial.
+
+  (* equ_sys_inv *)
+
+  apply H2. apply set_remove_3.
+  apply set_add_intro1; trivial.
+  discriminate.
+  assert (Q : c1 |- (pi++(! pi')|.X)|^s1 ~c ((([])|.X)|^s1)).
+   apply H3. apply set_remove_3.
+   apply set_add_intro2; trivial.
+   intro H5. inverts H5. apply H12; trivial.
+  case (Constraint_eqdec (s~?t) ((pi|.X)~?(pi'|.X))); intro H7. 
+  inverts H7. 
+  replace (pi|.X) with (pi @ ([]|.X)).
+  replace (pi'|.X) with (pi' @ ([]|.X)).  
+  rewrite 2 subst_perm_comm.
+  apply c_equiv_sym.
+  apply c_equiv_pi_inv_side.
+  apply c_equiv_sym.
+  rewrite perm_comp.
+  rewrite <- subst_perm_comm.
+  autorewrite with perm. simpl app; trivial.
+  autorewrite with perm; simpl; trivial.
+  autorewrite with perm; simpl; trivial. 
+  apply H3. apply set_remove_3; trivial.
+  apply set_add_intro1; trivial.
+
+Qed.
+
+
+Lemma tr_clos_equ_sol_preserv : forall T T' Sl varSet, valid_triple T ->
+      tr_clos _ (equ_sys varSet) T T' -> sol_c Sl T' -> sol_c Sl T .
+Proof.
+  intros. induction H0; trivial.
+  apply equ_sol_preserv with (Sl:=Sl) in H0; trivial.
+  apply equ_sol_preserv with (Sl:=Sl) in H0; trivial.
+  apply IHtr_clos; trivial.
+  apply equ_valid_preservation with (T:= s) (varSet:=varSet); trivial.
+Qed.
+  
+(** %\subsection{ Preservation of solutions by unif\_step }% *) 
+(**
+	Be a unifcation step form T to T'. If Sl is a solution
+	for T', then Sl is also a solution for T. This is proved
+	by case analysis over unif_step T T' and uses lemmas
+	fresh_sys_compl and equ_sol_preserv.
+*)
+
+Lemma unif_step_preserv : forall T T' Sl varSet,
+                          valid_triple T ->
+                          unif_step varSet T T' -> sol_c Sl T' -> sol_c Sl T.
+Proof.
+ intros. destruct H0.
+ apply equ_sol_preserv with (T':= T') (varSet:=varSet); trivial.
+ apply fresh_sys_compl with (Sl:=Sl) in H2. apply H2; trivial.
+Qed.
+
+ 
+(** %\subsection{ Soundness of the C-unification algorithm }% *)  
+(** 
+	Be a unifcation path form T to T'. If Sl is a solution
+	for T', then Sl is also a solution for T. This is proved
+	by case analysis over unif_path T T' and uses lemma
+	unif_step_preserv.
+*)
+ 
+Theorem c_unif_path_soundness : forall T T' Sl varSet,
+                                valid_triple T ->
+                                unif_path varSet T T' -> sol_c Sl T' -> sol_c Sl T.
+Proof.
+  intros. destruct H0.
+  induction H0; trivial.
+  apply unif_step_preserv with (Sl := Sl) in H0; trivial.
+  apply unif_step_preserv with (Sl := Sl) in H0; trivial.
+  apply IHtr_clos; trivial.
+  apply unif_step_valid_preserv with (T:= s) (varSet:=varSet); trivial.
+Qed.
+
+
+
+
+(** %\section{ Characterisation of successful leaves }% *)   
+(**
+	The characterisation of successful leaves is 
+	the subject of this part of the theory.
+
+*)
+
+(** % \subsection{ Freshness constraints in a leaf } % *)
+(**
+	Be a leaf T = (C, S, P). If [a#?s] is in P and the 
+	equational part of P is a fixpoint problem, then 
+	the term s must be equal to [a]. This statement 
+	is proved by case analysis over [s].
+*)
+
+Lemma leaf_fresh_sys : forall a s C S P varSet,
+                         set_In (a#?s) P ->
+                         leaf varSet (C,S,P) ->
+                         fixpoint_Problem (equ_proj P) ->
+                         s = %a.
+Proof.
+  intros. unfold leaf in H0. unfold NF in H0.
+  destruct s; trivial.
+  false. apply (H0 (C, S, P\(a #? (<<>>)))).
+  apply fresh_unif_step; trivial. apply fresh_sys_Ut; trivial.
+  case (a ==at a0); intro H2. rewrite H2; trivial.
+  false. apply (H0 (C, S, P\(a #? (%a0)))).
+  apply fresh_unif_step; trivial. apply fresh_sys_At; trivial. 
+  case (a ==at a0); intro H2. rewrite H2 in *|-.
+  false. apply (H0 (C, S, P\(a0 #? ([a0]^s)))).
+  apply fresh_unif_step; trivial. apply fresh_sys_Ab_1; trivial. 
+  false. apply (H0 (C, S, (P|+(a#?s))\(a #? ([a0]^s)))).
+  apply fresh_unif_step; trivial. apply fresh_sys_Ab_2; trivial. 
+  false. apply (H0 (C,S,(((P|+(a#?s1))|+(a#?s2))\(a#?(<|s1,s2|>))))).
+  apply fresh_unif_step; trivial. apply fresh_sys_Pr; trivial.
+  false. apply (H0 (C, S, (P|+(a#?s))\(a #? (Fc n n0 s)))).
+  apply fresh_unif_step; trivial. apply fresh_sys_Fc; trivial.
+  false. apply (H0 (C|++((!p) $ a,v),S,(P\(a#?(p|.v))))).  
+  apply fresh_unif_step; trivial. apply fresh_sys_Su; trivial.
+Qed.
+
+
+(** % \subsection{ Characterisation of equations that are in normal forms of equ\_sys } % *)
+(**
+	Be T = (C, S, P) a normal form regarding equ_sys. If s ~? t is in P then 
+	it must match with one of the following showed cases. This is proved by case analysis
+	over s and t. 
+	
+	Notice that the predicate Proper_Problem P synthesises
+	the following property: for each equation s ~? t in P, if s or t 
+	has as a subterm (Fc C n s0), with C commutative, then s0
+	must be a pair. This restriction was added to insure that
+	commutative function symbols are only applied to pairs.
+*)  
+
+Lemma NF_equ_sys : forall C S P varSet,
+                     
+           Proper_Problem P ->
+
+           NF _ (equ_sys varSet) (C, S, P) ->
+
+            (forall s t, set_In (s ~? t) P ->
+                        
+            ((forall pi X, t <> pi|.X) /\
+              ((s = (<<>>) /\ t <> (<<>>)) \/
+              (exists a, s = (%a) /\ t <> (%a))  \/
+              (exists E n u, s = (Fc E n u) /\ forall v, t <> (Fc E n v)) \/
+              (exists a u, s = [a]^u /\ forall b v, t <> [b]^v) \/
+              (exists u v, s = (<|u,v|>) /\ forall u' v', t <> (<|u',v'|>))  \/
+              (exists pi X, s = pi|.X /\ set_In X (set_union Var_eqdec (term_vars t) varSet)))) \/     
+            
+            ((forall pi X, s <> pi|.X) /\ (exists pi, exists X, t = pi|.X /\
+                                                 set_In X (set_union Var_eqdec (term_vars s) varSet)))
+               \/
+
+            (exists pi pi' X Y, X <> Y /\ s = pi|.X /\ t = pi'|.Y /\ set_In X varSet /\ set_In Y varSet) \/   
+               
+            (fixpoint_equ (s ~? t)) ).
+Proof.
+  intros.
+
+  case (term_eqdec s t); intro H2.
+  (* s = t *)
+   rewrite H2 in *|-*; clear H2. 
+   false. apply (H0 (C, S, P\(t~?t))). apply equ_sys_refl; trivial.                             
+  (* s <> t *)
+   case (Su_eqdec s); case (Su_eqdec t); intros H3 H4.
+   (* s and t are both suspensions *)  
+    case H3; clear H3; intros pi' H3. case H3; clear H3; intros Y H3.
+    case H4; clear H4; intros pi H4. case H4; clear H4; intros X H4.
+    rewrite H3 in *|-*. rewrite H4 in *|-*. clear H3 H4.
+    case (Y ==v X); intro H3. 
+     (* the variables of the two suspesions are equal *)
+      rewrite H3 in *|-*. clear H3.
+      case (Perm_eqdec pi' ([])); intro H3.
+      (* pi' = [] *) 
+       rewrite H3 in *|-*. clear H3. 
+       right~. right~. right~. unfold fixpoint_equ. exists pi X.
+       split~. intro H3. rewrite H3 in H2. false. 
+      (* pi' <> [] *)
+       false. apply (H0 (C,S,(P|+((pi++(!pi'))|.X~?([]|.X)))\((pi|.X)~?(pi'|.X)))).
+       apply equ_sys_inv; trivial. intro H4. rewrite H4 in H2. false.    
+     (* the variables of the two suspesions are different *) 
+       case (set_In_dec Var_eqdec X varSet); intro H4.
+       (* X is in varSet *)
+        case (set_In_dec Var_eqdec Y varSet); intro H5.
+        (* Y is in varSet *)
+         right~. right~. left~. exists pi pi' X Y. repeat split~.
+        (* Y is not in varSet *) 
+         false.
+          apply (H0 (C,S©([(Y,(!pi')@(pi|.X))]),
+                        ((P\(pi'|.Y~?(pi|.X))\((pi|.X)~?(pi'|.Y)))|^^([(Y,(!pi')@(pi|.X))]))
+                          \cup(C/?(S©([(Y,(!pi')@(pi|.X))]))))).
+          apply equ_sys_inst; trivial. simpl. intro H6.
+          apply set_union_elim in H6. destruct H6; try contradiction.
+          simpl in H6. destruct H6; trivial. symmetry in H6. contradiction.
+          right~.
+       false.
+         apply (H0 (C,S©([(X,(!pi)@(pi'|.Y))]),
+                        ((P\(pi|.X~?(pi'|.Y))\((pi'|.Y)~?(pi|.X)))|^^([(X,(!pi)@(pi'|.Y))]))
+                          \cup(C/?(S©([(X,(!pi)@(pi'|.Y))]))))).
+       apply equ_sys_inst; trivial. simpl. intro H5.
+       apply set_union_elim in H5. destruct H5; try contradiction.
+       simpl in H5. destruct H5; trivial. contradiction.
+       left~.
+   (* only s is a suspension *)
+    case H4; clear H4; intros pi H4.    
+    case H4; clear H4; intros X H4. rewrite H4 in *|-*. clear H4.
+    case (set_In_dec Var_eqdec X (set_union Var_eqdec (term_vars t) varSet)); intro H4.
+    (* X is in set_union _ (term_vars t) varSet *)
+     left~. split~. right~. right~. right~. right~. right~.
+     exists pi X. split~.
+    (* X is not in set_union _ (term_vars t) varSet *) 
+     false. apply (H0 (C,S©([(X,(!pi)@t)]),
+                        ((P\(pi|.X~?t)\(t~?(pi|.X)))|^^([(X,(!pi)@t)]))
+                          \cup(C/?(S©([(X,(!pi)@t)]))))).
+     apply equ_sys_inst; trivial. left~.
+   (* only t is a suspension *)  
+    case H3; clear H3; intros pi H3.    
+    case H3; clear H3; intros X H3. rewrite H3 in *|-*. clear H3.
+    case (set_In_dec Var_eqdec X (set_union Var_eqdec (term_vars s) varSet)); intro H5.
+    (* X is in set_union _ (term_vars s) varSet *)
+     right~. left~. split~. exists pi X. split~.     
+    (* X is not in set_union _ (term_vars s) varSet *)
+     false. apply (H0 (C,S©([(X,(!pi)@s)]),
+                        ((P\(pi|.X~?s)\(s~?(pi|.X)))|^^([(X,(!pi)@s)]))
+                          \cup(C/?(S©([(X,(!pi)@s)]))))).
+     apply equ_sys_inst; trivial. right~.
+
+  (* both s and t are not suspensions *)
+   left~. split~. destruct s.
+   (* s = <<>> *)
+    left~.
+   (* s = %a *)
+    right~. left~. exists a. split~.
+   (* s = [a]^s0 *)
+    right~. right~. right~. left~. 
+    exists a. exists s. split~; intros.
+    intro H5. rewrite H5 in *|-*; clear H5.
+    case (a ==at b); intro H5. rewrite H5 in H1.
+    apply (H0 (C,S,P|+(s~?v)\(([b]^s)~?([b]^v)))).
+    apply equ_sys_Ab1; trivial. 
+    apply (H0 (C,S,((P|+(s~?([(a,b)]@v))|+(a#?v)))\(([a]^s)~?([b]^v)))).
+    apply equ_sys_Ab2; trivial. 
+   (* s = <|s1, s2|> *)
+    right~. right~. right~. right~. left~.
+    exists s1 s2. split~; intros. intro H5.
+    rewrite H5 in *|-*.
+    apply (H0 (C,S,((P|+(s1~?u'))|+(s2~?v'))\(<|s1, s2|>~?<|u', v'|>))).
+    apply equ_sys_Pr; trivial.
+   (* s = Fc n n0 s0 *) 
+    right~. right~. left~. exists n n0 s. split~; intros.
+    intro H5. rewrite H5 in *|-*. clear H5.
+    case (eq_nat_dec n 2); intro H5. rewrite H5 in *|-*; clear H5.
+    assert (Q : is_Pr s /\ is_Pr v).
+     apply H in H1. destruct H1.
+     unfold Proper_term in H1.
+     unfold Proper_term in H5. split~.
+     apply H1 with (n:=n0). apply In_subterms.
+     apply H5 with (n:=n0). apply In_subterms.
+    destruct Q. apply is_Pr_exists in H5. apply is_Pr_exists in H6.
+    case H5; clear H5; intros s0 H5. case H5; clear H5; intros s1 H5.
+    case H6; clear H6; intros t0 H6. case H6; clear H6; intros t1 H6.
+    rewrite H5 in *|-. rewrite H6 in *|-*. clear H5 H6.
+    apply (H0 (C,S,((P|+(s0~?t0))|+(s1~?t1))\(Fc 2 n0 (<|s0,s1|>)~?(Fc 2 n0 (<|t0,t1|>))))).
+    apply equ_sys_C1; trivial.
+    apply (H0 (C,S,(P|+(s~?v))\(Fc n n0 s ~?(Fc n n0 v)))).
+    apply equ_sys_Fc; trivial.
+
+   false. 
+ 
+Qed.
+
+
+(** % \subsection{ Equations in a sucessful leaf by equ\_sys } % *)
+(**
+	Be T = (C, S, P) a normal form of equ_sys. If s ~? t is in P and 
+	T has solutions, then s ~? t must be a fixpoint equation. 
+	A proof of this lemma is obtained by case analysis over the feasible
+	normal forms of equ_sys, and it uses Lemma NF_equ_sys.
+*)
+
+Lemma NF_successful_equ: forall C S P s t varSet,
+                         Proper_Problem P ->
+                         set_In (s ~? t) P -> 
+                         NF _ (equ_sys varSet) (C, S, P) ->
+                         (exists Sl, sol_c Sl (C, S, P) /\
+                          set_inter Var_eqdec (dom_rec (snd Sl)) varSet = []) -> 
+                         fixpoint_equ (s ~? t).  
+Proof.
+  intros. case H2; clear H2; intros Sl H2. destruct H2.
+  unfold sol_c in H2.
+  destruct H2. destruct H4. destruct H5. simpl fst in *|-. simpl snd in *|-.
+  apply NF_equ_sys with (s:=s) (t:=t) (varSet := varSet) in H1; trivial.
+  destruct H1. destruct H1. destruct H7. destruct H7.
+  assert (Q : fst Sl |- (<<>>) |^ snd Sl ~c (t |^ snd Sl)). 
+   rewrite <- H7. apply H5; trivial.
+  inverts Q. false. apply H8.
+  destruct t; simpl in H10; inverts H10; trivial. false.   
+  destruct H7. case H7; clear H7; intros a H7. destruct H7.   
+  assert (Q : fst Sl |- (%a) |^ snd Sl ~c (t |^ snd Sl)). 
+   rewrite <- H7. apply H5; trivial. 
+  inverts Q. false. apply H8.
+  destruct t; simpl in H12; inverts H12; trivial. false. 
+  destruct H7. case H7; clear H7; intros E H7.
+  case H7; clear H7; intros n H7.
+  case H7; clear H7; intros u H7. destruct H7.  
+  assert (Q : fst Sl |- (Fc E n u) |^ snd Sl ~c (t |^ snd Sl)). 
+   rewrite <- H7. apply H5; trivial. 
+  inverts Q. destruct t; simpl in H14; inverts H14; trivial.
+  false. false. simpl in H14. omega. simpl in H14. omega.
+  destruct t; simpl in H13; inverts H13. false. false.
+  destruct t; simpl in H13; inverts H13. false. false.  
+  destruct H7. 
+  case H7; clear H7; intros a H7.
+  case H7; clear H7; intros u H7. destruct H7.  
+  assert (Q : fst Sl |- ([a]^u) |^ snd Sl ~c (t |^ snd Sl)). 
+   rewrite <- H7. apply H5; trivial. 
+  inverts Q. destruct t; simpl in H13; inverts H13;
+   trivial. false. false. destruct t; inverts H11. false. false.
+  destruct H7.
+  case H7; clear H7; intros u H7.
+  case H7; clear H7; intros v H7. destruct H7.
+  assert (Q : fst Sl |- (<|u,v|>) |^ snd Sl ~c (t |^ snd Sl)). 
+   rewrite <- H7. apply H5; trivial. 
+  inverts Q. destruct t; simpl in H12; inverts H12;
+   trivial. false. false.
+  case H7; clear H7; intros pi H7.
+  case H7; clear H7; intros X H7. destruct H7.
+  assert (Q : fst Sl |- (pi|.X) |^ snd Sl ~c (t |^ snd Sl)). 
+   rewrite <- H7. apply H5; trivial.
+  apply set_union_elim in H8. destruct H8.
+  assert (Q' : set_In X (term_vars ((!pi) @ t))).
+   rewrite perm_term_vars; trivial.
+  apply psubterms_subs with (S:=snd Sl) in Q'; trivial.
+  case Q'; clear Q'; intros pi' Q'.
+  replace (pi|.X) with (pi @ ([]|.X)) in Q;
+  autorewrite with perm; trivial. 
+  rewrite subst_perm_comm in Q.
+  apply c_equiv_pi_inv_side in Q.
+  apply c_equiv_perm_psubterm with (pi := pi') in Q.
+  rewrite <- 2 subst_perm_comm in Q.
+  autorewrite with perm in Q. simpl app in Q.
+  contradiction.
+  intros. intro H9. destruct t;
+    autorewrite with perm in H9; inverts H9. false.
+  rewrite inter_dom_term_vars in Q. inverts Q.
+  destruct t; simpl in H13; inverts H13. false.
+  apply set_inter_nil. intros Y H9.
+  apply set_inter_nil with (a:=Y) in H3.
+  apply H3. clear H3. apply set_inter_elim in H9.
+  destruct H9. simpl in H3. destruct H3; try contradiction.
+  apply set_inter_intro; trivial.
+  rewrite <- H3; trivial.
+  destruct H1. destruct H1.
+  case H7; clear H7; intros pi H7.
+  case H7; clear H7; intros X H7. destruct H7.
+  assert (Q : fst Sl |- s |^ snd Sl ~c ((pi|.X) |^ snd Sl)). 
+   rewrite <- H7. apply H5; trivial.
+  apply set_union_elim in H8. destruct H8.
+  assert (Q' : set_In X (term_vars ((!pi) @ s))).
+   rewrite perm_term_vars; trivial. apply c_equiv_sym in Q.
+  apply psubterms_subs with (S:=snd Sl) in Q'; trivial.
+  case Q'; clear Q'; intros pi' Q'.
+  replace (pi|.X) with (pi @ ([]|.X)) in Q;
+  autorewrite with perm; trivial. 
+  rewrite subst_perm_comm in Q.
+  apply c_equiv_pi_inv_side in Q.
+  apply c_equiv_perm_psubterm with (pi := pi') in Q.
+  rewrite <- 2 subst_perm_comm in Q.
+  autorewrite with perm in Q. simpl app in Q.
+  contradiction.
+  intros. intro H9. destruct s;
+    autorewrite with perm in H9; inverts H9. false.
+  rewrite inter_dom_term_vars with (t:=pi|.X) in Q. inverts Q.
+  destruct s; simpl in H9; inverts H9. false.
+  apply set_inter_nil. intros Y H9.
+  apply set_inter_nil with (a:=Y) in H3.
+  apply H3. clear H3. apply set_inter_elim in H9.
+  destruct H9. simpl in H3. destruct H3; try contradiction.
+  apply set_inter_intro; trivial.
+  rewrite <- H3; trivial.
+  destruct H1; trivial.
+  case H1; clear H1; intros pi H1.
+  case H1; clear H1; intros pi' H1.
+  case H1; clear H1; intros X H1.  
+  case H1; clear H1; intros Y H1.
+  destruct H1. destruct H7. destruct H8. destruct H9.
+  apply H5 in H0. rewrite H7 in H0. rewrite H8 in H0.
+  rewrite 2 inter_dom_term_vars in H0.
+  inverts H0. false.
+  apply set_inter_nil; intros Z H11.
+  apply set_inter_nil with (a:=Z) in H3.
+  apply H3; clear H3.
+  apply set_inter_elim in H11. destruct H11.
+  simpl in H3. destruct H3; try contradiction.
+  apply set_inter_intro; trivial. rewrite <- H3; trivial.
+  apply set_inter_nil; intros Z H11.
+  apply set_inter_nil with (a:=Z) in H3.
+  apply H3; clear H3.
+  apply set_inter_elim in H11. destruct H11.
+  simpl in H3. destruct H3; try contradiction.
+  apply set_inter_intro; trivial. rewrite <- H3; trivial.
+  
+Qed.
+
+
+(** % \subsection{ Characterisation of successful leaves } % *)
+(**
+		A successful leaf T = (C, S, P) must be a fixpoint problem. This
+		is proved by case analysis over P, and 
+		uses lemmas NF_successful_equ and leaf_fresh_sys.
+*)
+  
+Lemma successful_leaves_ch : forall T varSet,
+                               Proper_Problem (snd T) ->
+                               (leaf varSet T /\
+                                (exists Sl, (sol_c Sl T) /\
+                                 set_inter Var_eqdec (dom_rec (snd Sl)) varSet = [] )) ->
+                               (fixpoint_Problem (snd T)).
+Proof.
+  intros. destruct H0. 
+  destruct T. destruct p. simpl.
+  
+  assert (Q : fixpoint_Problem (equ_proj p0)).
+   apply set_In_fixpoint_eq_proj; intros.   
+   apply NF_successful_equ with (C:=c) (S:=s) (P:=p0) (varSet:=varSet); trivial.
+   unfold leaf in H0. unfold NF in *|-*.
+   intros T H3. apply (H0 T). apply equ_unif_step; trivial.
+
+  unfold fixpoint_Problem; intros. destruct u.
+
+  case H1; clear H1; intros Sl H1. unfold sol_c in H1.  
+  destruct H1. destruct H1. destruct H4.
+  apply leaf_fresh_sys with (a:=a) (s:=t) in H0; trivial.    
+  assert (Q': fst Sl |- a # ((%a) |^ snd Sl)).  
+   apply H4. simpl. rewrite <- H0. trivial.
+  simpl in Q'. inverts Q'. false.
+   
+  apply NF_successful_equ with (C:=c) (S:=s) (P:=p0) (varSet:=varSet); trivial.
+  unfold leaf in H0. unfold NF in *|-*.
+  intros T H3. apply (H0 T).   
+  apply equ_unif_step; trivial.
+Qed.    
+
+
+(** % \subsection{ Generated successful leaves } % *)
+(** 
+	Be a unification path from T to T'. If T' = (C', S', P') is
+	a successful leaf, then P' is a fixpoint problem. This is 
+	a corollary of the Lemma successful_leaves_ch.
+*)	
+
+Corollary gen_successfull_leaves : forall T T' varSet,                              
+                                   Proper_Problem (snd T)  ->
+                                   unif_path varSet T T' ->  
+                                    (exists Sl, (sol_c Sl T') /\
+                                     set_inter Var_eqdec (dom_rec (snd Sl)) varSet = []) ->   
+                                   fixpoint_Problem (snd T').
+Proof.
+  intros. apply successful_leaves_ch with (varSet:=varSet).
+  apply unif_path_Proper_Problem with (T:=T) (varSet:=varSet); trivial.
+  destruct H0. split~.
+Qed.
